## Taylor function

$f(x) = f(x_{0})+\frac{f^{1}(x_{0})}{1!}+\frac{f^{2}(x_{0})}{2!}+\cdots+\frac{f^{(n)}(x_{0})}{n!}$       $\sum_{n=0}^{n=\infty} \frac{f^{(n)}(x_{0})}{n!}$

$e^{x} = 1 + \frac{x}{1!} + \frac{x^{2}}{2!} + \cdots+ \frac{x^n}{n!}$

$\frac{1}{1-x} = 1 + x +x^{2} +x^{3} +\cdots+x^{n}$ (Sum by equal ratio)

$\frac{1}{1+x} = 1 -x+x^{2}-x^{3}+\cdots+(-1)^{n}x^{n} $

$sinx = \sum_{n=0}^{n=\infty} (-1)^{n}\frac{x^{2n+1}}{(2n+1)!}$

$cosx = \sum_{n=0}^{n=\infty} (-1)^{n}\frac{x^{2n}}{(2n)!}$

$ln(1+x) = \sum_{n=1}^{n=\infty}(-1)^{n}\frac{x^{n}}{n}$ $\frac{1}{1+x}$ integral

$ln(1-x) = \sum_{n=1}^{n=\infty} \frac{x^{n}}{n}$
